lifted nat restriction

theories/Borda_Rule_Ref.thy
@@ -5,15 +5,32 @@ theory Borda_Rule_Ref
 begin
 
 definition borda_rule_sep where
-  "borda_rule_sep A p \<equiv> elector_sep borda_elim_sep (A, p)"
-
-interpretation borda_rule_impl: elector_ref borda_ref borda_elim_sep borda
-  apply unfold_locales
+  "borda_rule_sep \<equiv> elector_sep borda_elim_sep"
+                                   
+interpretation borda_rule_impl: elector_sepref borda_ref borda_elim_sep borda
+  apply unfold_locales            
   subgoal using borda_elim_sep.refine .
   subgoal using borda_sound .
   subgoal apply (intro frefI) using borda_ref_correct[THEN frefD] by auto
   done
 
-lemmas borda_rule_correct = borda_rule_impl.elector_sep_correct
+lemmas borda_rule_correct_aux  = borda_rule_impl.elector_sep_correct
 
+lemma  borda_rule_correct:
+  shows "(borda_rule_sep, uncurry (RETURN oo borda_rule))
+    \<in> [\<lambda>(A, pl).
+           finite_profile A
+            pl]\<^sub>a (hr_comp (hs.assn id_assn) (\<langle>Id\<rangle>set_rel))\<^sup>k *\<^sub>a
+                  (list_assn
+                    (hr_comp ballot_impl_assn
+                      ballot_rel))\<^sup>k \<rightarrow> hr_comp (hs.assn id_assn) (\<langle>Id\<rangle>set_rel) \<times>\<^sub>a
+                                        hr_comp (hs.assn id_assn) (\<langle>Id\<rangle>set_rel) \<times>\<^sub>a
+                                        hr_comp (hs.assn id_assn) (\<langle>Id\<rangle>set_rel)"
+  unfolding borda_rule_sep_def borda_rule.simps using borda_rule_correct_aux .
+
+
+export_code borda_rule_sep in Scala_imp
+
+definition "ttest == borda_rule_sep hs. "
+                                          
 end
