theories/Compositional_Structures/Elect_Composition_Ref.thy
@@ -11,7 +11,7 @@ definition
 thm "elector_sep_def"
 
 locale elector_impl =  
-  fixes m_ref :: "'a::{default, linorder, hashable, heap} Electoral_Module_Ref"
+  fixes m_ref :: "'a::{default, hashable, heap} Electoral_Module_Ref"
   fixes m_sep :: "('a, unit) hashtable
       \<Rightarrow> ('a array \<times> nat) list
          \<Rightarrow> (('a, unit) hashtable \<times> ('a, unit) hashtable \<times> ('a, unit) hashtable) Heap"
@@ -20,18 +20,18 @@ locale elector_impl =
         \<in> (alts_set_impl_assn)\<^sup>k *\<^sub>a profile_impl_assn\<^sup>k \<rightarrow>\<^sub>a result_impl_assn"
 
 
-locale elector_ref = elector_impl +
-  fixes m :: "nat Electoral_Module"
+locale elector_sepref = elector_impl +
+  fixes m :: "'a::{default, hashable, heap}  Electoral_Module"
 assumes module_m: "electoral_module m"
 assumes m_ref_correct: "(uncurry m_ref, uncurry (RETURN oo m)) \<in> 
   ([\<lambda> (A, pl). finite_profile A
-            pl]\<^sub>f (\<langle>nat_rel\<rangle>set_rel \<times>\<^sub>r profile_rel)
-   \<rightarrow> \<langle>\<langle>nat_rel\<rangle>set_rel \<times>\<^sub>r \<langle>nat_rel\<rangle>set_rel \<times>\<^sub>r \<langle>nat_rel\<rangle>set_rel\<rangle>nres_rel)" 
+            pl]\<^sub>f (\<langle>Id\<rangle>set_rel \<times>\<^sub>r profile_rel)
+   \<rightarrow> \<langle>\<langle>Id\<rangle>set_rel \<times>\<^sub>r \<langle>Id\<rangle>set_rel \<times>\<^sub>r \<langle>Id\<rangle>set_rel\<rangle>nres_rel)" 
 begin
 
 lemmas m_t_ref = m_impl[FCOMP m_ref_correct]
 
-interpretation elector: sequence_refine m_ref m_sep elect_module_ref elect_module_sep m elect_module
+interpretation elector: sequence_sepref m_ref m_sep elect_module_ref elect_module_sep m elect_module
   apply unfold_locales
   subgoal using m_impl .
   subgoal  using elect_module_sep.refine .
@@ -46,9 +46,22 @@ interpretation elector: sequence_refine m_ref m_sep elect_module_ref elect_modul
 interpretation elector:  seqcomp_impl m_ref m_sep elect_module_ref elect_module_sep
   apply unfold_locales .
 
-lemmas elector_sep_refine =  elector.seqt_sep_refine
 
-lemmas elector_sep_correct =  elector.sequence_correct
+lemmas elector_sep_correct_aux =  elector.sequence_correct
+
+lemma elector_sep_correct:
+  shows "(elector_sep m_sep, uncurry (RETURN oo elector m))
+\<in> [\<lambda>(A, pl).
+           finite_profile A pl]\<^sub>a 
+  (hr_comp (hs.assn id_assn) (\<langle>Id\<rangle>set_rel))\<^sup>k *\<^sub>a
+                 (list_assn
+                   (hr_comp ballot_impl_assn
+                     ballot_rel))\<^sup>k \<rightarrow> hr_comp (hs.assn id_assn) (\<langle>Id\<rangle>set_rel) \<times>\<^sub>a
+                                       hr_comp (hs.assn id_assn) (\<langle>Id\<rangle>set_rel) \<times>\<^sub>a
+                                       hr_comp (hs.assn id_assn) (\<langle>Id\<rangle>set_rel)"
+  unfolding elector_sep_def elector.simps 
+  using elector_sep_correct_aux by simp
+
 
 end
 
