theories/Compositional_Structures/Sepref_Bindings.thy
@@ -29,35 +29,57 @@ sepref_decl_op (no_def) "borda :: 'a Electoral_Module" :: "elec_mod_rel_orig Id"
   using borda_aux .
 
 
-
 sepref_decl_op (no_def) defer_equal_imp: "(defer_equal_condition)" :: 
   "\<langle>nat_rel, \<langle>(\<langle>R\<rangle>set_rel \<times>\<^sub>r \<langle>R\<rangle>set_rel \<times>\<^sub>r \<langle>R\<rangle>set_rel), \<langle>bool_rel\<rangle>nres_rel\<rangle>fun_rel\<rangle>fun_rel" 
   where "R = Id" .
 
 
 
+                              
+
+definition "alts_ref_assn \<equiv> hr_comp alts_set_impl_assn (\<langle>Id\<rangle>set_rel)"
+                                 
+
+definition "ballot_ref_assn \<equiv>  hr_comp (ballot_impl_assn) (\<langle>Id\<rangle>list_rel)"
+
+definition "alts_assn \<equiv> hr_comp alts_ref_assn (\<langle>Id\<rangle>set_rel)"
+
+definition "result_set_one_step \<equiv> hr_comp alts_set_impl_assn (\<langle>Id\<rangle>set_rel)"
+
+definition "result_set_assn \<equiv> hr_comp(result_set_one_step) (\<langle>Id\<rangle>set_rel)"
+
+definition "ballot_assn \<equiv> hr_comp (hr_comp (ballot_impl_assn) ballot_rel) (\<langle>Id \<times>\<^sub>r Id\<rangle>set_rel)"
 
 
 locale refine_assns =
  notes  
        ballot_assn_def[symmetric,fcomp_norm_unfold]
        result_set_assn_def[symmetric,fcomp_norm_unfold]
-       alts_ref_assn_def[symmetric,fcomp_norm_unfold] ballot_ref_assn_def[symmetric,fcomp_norm_unfold]
+       alts_ref_assn_def[symmetric,fcomp_norm_unfold] 
+       ballot_ref_assn_def[symmetric,fcomp_norm_unfold]
        alts_assn_def[symmetric,fcomp_norm_unfold] 
        result_set_one_step_def[symmetric,fcomp_norm_unfold]
       
 begin
 
 
-sepref_decl_impl borda_impl: borda_elim_sepref.refine[FCOMP borda_ref_correct] 
+sepref_decl_impl borda_impl: borda_elim_sep.refine[FCOMP borda_ref_correct] 
   by simp                                       
 
-
+         
 
 sepref_decl_impl defer_eqal_condition_impl: defer_equal_condition_sep.refine .
 
+ definition "funsc A p \<equiv> RETURN (borda A p)"
+
+ sepref_definition first_imple 
+    is "uncurry funsc" :: "unit_assn\<^sup>k \<rightarrow>\<^sub>a  (alts_assn \<times>\<^sub>a alts_assn \<times>\<^sub>a alts_assn) "
+   unfolding funsc_def id_def comp_def
+   apply sepref_dbg_keep
+
+
 end
 
-  
+
 
 end
